.

src/Init/Data/Array/Attach.lean
@@ -5,6 +5,7 @@ Authors: Joachim Breitner, Mario Carneiro
 -/
 prelude
 import Init.Data.Array.Mem
+import Init.Data.Array.Lemmas
 import Init.Data.List.Attach
 
 namespace Array
@@ -26,4 +27,127 @@ Unsafe implementation of `attachWith`, taking advantage of the fact that the rep
   with the same elements but in the type `{x // x ∈ xs}`. -/
 @[inline] def attach (xs : Array α) : Array {x // x ∈ xs} := xs.attachWith _ fun _ => id
 
-end Array
+@[simp] theorem _root_.List.attachWith_toArray {l : List α} {P : α → Prop} {H : ∀ x ∈ l.toArray, P x} :
+    l.toArray.attachWith P H = (l.attachWith P (by simpa using H)).toArray := by
+  simp [attachWith]
+
+@[simp] theorem _root_.List.attach_toArray {l : List α} :
+    l.toArray.attach = (l.attachWith (· ∈ l.toArray) (by simp)).toArray := by
+  simp [attach]
+
+@[simp] theorem toList_attachWith {l : Array α} {P : α → Prop} {H : ∀ x ∈ l, P x} :
+   (l.attachWith P H).toList = l.toList.attachWith P (by simpa [mem_toList] using H) := by
+  simp [attachWith]
+
+@[simp] theorem toList_attach {α : Type _} {l : Array α} :
+    l.attach.toList = l.toList.attachWith (· ∈ l) (by simp [mem_toList]) := by
+  simp [attach]
+
+/-! ## unattach
+
+`Array.unattach` is the (one-sided) inverse of `Array.attach`. It is a synonym for `Array.map Subtype.val`.
+
+We use it by providing a simp lemma `l.attach.unattach = l`, and simp lemmas which recognize higher order
+functions applied to `l : Array { x // p x }` which only depend on the value, not the predicate, and rewrite these
+in terms of a simpler function applied to `l.unattach`.
+
+Further, we provide simp lemmas that push `unattach` inwards.
+-/
+
+/--
+A synonym for `l.map (·.val)`. Mostly this should not be needed by users.
+It is used introduced as in intermediate step by lemmas such as `map_subtype`,
+and is ideally subsequently simplified away by `unattach_attach`.
+
+If not, usually the right approach is `simp [Array.unattach, -Array.map_subtype]` to unfold.
+-/
+def unattach {α : Type _} {p : α → Prop} (l : Array { x // p x }) := l.map (·.val)
+
+@[simp] theorem unattach_nil {α : Type _} {p : α → Prop} : (#[] : Array { x // p x }).unattach = #[] := rfl
+@[simp] theorem unattach_push {α : Type _} {p : α → Prop} {a : { x // p x }} {l : Array { x // p x }} :
+    (l.push a).unattach = l.unattach.push a.1 := by
+  simp [unattach]
+
+@[simp] theorem size_unattach {α : Type _} {p : α → Prop} {l : Array { x // p x }} :
+    l.unattach.size = l.size := by
+  unfold unattach
+  simp
+
+-- @[simp] theorem _root_.List.unattach_toArray {α : Type _} {p : α → Prop} {l : List { x // p x }} :
+--     l.toArray.unattach = l.unattach.toArray := by
+--   simp [unattach]
+
+-- @[simp] theorem toList_unattach {α : Type _} {p : α → Prop} {l : Array { x // p x }} :
+--     l.unattach.toList = l.toList.unattach := by
+--   simp [unattach]
+
+-- @[simp] theorem unattach_attach {α : Type _} (l : Array α) : l.attach.unattach = l := by
+--   cases l
+--   simp
+
+-- @[simp] theorem unattach_attachWith {α : Type _} {p : α → Prop} {l : Array α}
+--     {H : ∀ a ∈ l, p a} :
+--     (l.attachWith p H).unattach = l := by
+--   cases l
+--   simp
+
+-- /-! ### Recognizing higher order functions using a function that only depends on the value. -/
+
+-- /--
+-- This lemma identifies folds over arrays of subtypes, where the function only depends on the value, not the proposition,
+-- and simplifies these to the function directly taking the value.
+-- -/
+-- @[simp] theorem foldl_subtype {p : α → Prop} {l : Array { x // p x }}
+--     {f : β → { x // p x } → β} {g : β → α → β} {x : β}
+--     {hf : ∀ b x, f b x = g b x.1} :
+--     l.foldl f x = l.unattach.foldl g x := by
+--   cases l
+--   simp [hf]
+
+-- /--
+-- This lemma identifies folds over arrays of subtypes, where the function only depends on the value, not the proposition,
+-- and simplifies these to the function directly taking the value.
+-- -/
+-- @[simp] theorem foldr_subtype {p : α → Prop} {l : Array { x // p x }}
+--     {f : { x // p x } → β → β} {g : α → β → β} {x : β}
+--     {hf : ∀ x b, f x b = g x.1 b} :
+--     l.foldr f x = l.unattach.foldr g x := by
+--   cases l
+--   simp [hf]
+
+-- /--
+-- This lemma identifies maps over arrays of subtypes, where the function only depends on the value, not the proposition,
+-- and simplifies these to the function directly taking the value.
+-- -/
+-- @[simp] theorem map_subtype {p : α → Prop} {l : Array { x // p x }}
+--     {f : { x // p x } → β} {g : α → β} {hf : ∀ x, f x = g x.1} :
+--     l.map f = l.unattach.map g := by
+--   cases l
+--   simp [hf]
+
+-- @[simp] theorem filterMap_subtype {p : α → Prop} {l : Array { x // p x }}
+--     {f : { x // p x } → Option β} {g : α → Option β} {hf : ∀ x, f x = g x.1} :
+--     l.filterMap f = l.unattach.filterMap g := by
+--   cases l
+--   simp [hf]
+
+-- @[simp] theorem filter_unattach {p : α → Prop} {l : Array { x // p x }}
+--     {f : { x // p x } → Bool} {g : α → Bool} {hf : ∀ x, f x = g x.1} :
+--     (l.filter f).unattach = l.unattach.filter g := by
+--   cases l
+--   simp [hf]
+
+-- /-! ### Simp lemmas pushing `unattach` inwards. -/
+
+-- @[simp] theorem reverse_unattach {p : α → Prop} {l : Array { x // p x }} :
+--     l.reverse.unattach = l.unattach.reverse := by
+--   cases l
+--   simp
+
+-- @[simp] theorem append_unattach {p : α → Prop} {l₁ l₂ : Array { x // p x }} :
+--     (l₁ ++ l₂).unattach = l₁.unattach ++ l₂.unattach := by
+--   cases l₁
+--   cases l₂
+--   simp
+
+-- end Array
